examples/CADP_Bisimilarity.v
@@ -1,0 +1,150 @@
+Require Import MEBI.Examples.CADP.
+
+(* https://rocq-prover.org/doc/v8.9/stdlib/Coq.Relations.Relation_Operators.html *)
+Require Import Relation_Definitions.
+(* Variable R1 : relation M. *)
+
+Set Primitive Projections.
+
+Section Definitions.
+  Context
+    {M : Type}        (* term of lts 1 *)
+    {N : Type}        (* term of lts 2 *)
+    {A : Type}        (* actions of lts *)
+    (TAU : A -> Prop) (* determine if [A] is silent -- for weak *)
+    (LTS1 : M -> A -> M -> Prop)
+    (LTS2 : N -> A -> N -> Prop).
+
+  Definition simF (Sim : M -> N -> Prop) (s : M) (t : N) : Prop :=
+    forall s' a,
+      LTS1 s a s' ->
+      exists t',
+        LTS2 t a t' /\ Sim s' t'.
+
+  CoInductive sim (s : M) (t : N) : Prop :=
+    In_sim { out_sim :  simF sim s t }.
+
+
+  (* weak transitions -- refl & trans closure of tau transitions *)
+  (* prop holds *)
+  Inductive weak_refltr1 (lhs : Prop) (s : M) : Prop :=
+  | ltau1 : forall a s',
+      (TAU a -> True) /\ LTS1 s a s' /\ (lhs -> True) ->
+      weak_refltr1 lhs s' -> weak_refltr1 lhs s
+  | rtau1 : forall a s',
+      (TAU a -> True) /\ LTS1 s a s' /\ (lhs -> False) ->
+      weak_refltr1 lhs s' -> weak_refltr1 lhs s
+  | act1 : forall a s',
+      (TAU a -> False) /\ LTS1 s a s' /\ (lhs -> True) ->
+      weak_refltr1 False s' -> weak_refltr1 lhs s
+  | none1 : forall a s', LTS1 s a s'
+  .
+
+  (* Inductive weak_comptr1 (s : M) (a : A) : Prop :=
+  | comp : forall s',
+      weak_refltr1 True  *)
+
+
+  (* same as above, but for lts2 *)
+  Inductive weak_refltr2 (lhs:Prop) (s : N) : Prop :=
+  | ltau2 : forall a s',
+      (TAU a -> True) /\ LTS2 s a s' /\ (lhs -> True) ->
+      weak_refltr2 lhs s' -> weak_refltr2 lhs s
+  | rtau2 : forall a s',
+      (TAU a -> True) /\ LTS2 s a s' /\ (lhs -> False) ->
+      weak_refltr2 lhs s' -> weak_refltr2 lhs s
+  | act2 : forall a s',
+      (TAU a -> False) /\ LTS2 s a s' /\ (lhs -> True) ->
+      weak_refltr2 False s' -> weak_refltr2 lhs s
+  | none2 : forall a s', LTS2 s a s'
+  .
+
+  (* Definition weak_tr () *)
+
+
+  (* | rtau1 : forall s a s',
+      TAU a /\ LTS1 s a s' -> *)
+
+
+
+  (* weak sim *)
+  (* Definition wsimF (Sim : M -> N -> Prop) (s : M) (t : N) : Prop :=
+    forall s' a,
+    LTS1 s a s' ->
+      () *)
+
+
+  CoInductive wsim (s : M) (t : N) : Prop :=
+    In_wsim { out_wsim :  wsimF wsim s t }.
+
+
+End Definitions.
+
+Lemma sim_refl (M A : Type) (LTS : M -> A -> M -> Prop) (m : M)
+  : sim LTS LTS m m.
+Proof.
+  revert m.
+  cofix CH.
+  intros m.
+  constructor.
+  intros m' a tr.
+  exists m'.
+  split.
+  - exact tr.
+  - apply CH. Guarded.
+Qed.
+
+
+(* weak transition *)
+Definition tau_tr (a:CADP.action) : Prop := 
+  match a with 
+  | SILENT => True
+  | _ => False 
+  end.
+
+Lemma weak_bisim 
+  (* changed from [Set] to [Type] due to error. *) 
+  (* -- uncertain of impact, but recall D.CP. preferring [Set] *)
+  (M N A : Type) 
+  (LTS1 : M -> A -> M -> Prop)
+  (LTS2 : N -> A -> N -> Prop)
+  (m : M) (n : N) : weak_sim lts bigstep tau_tr g1 g1.
+Proof.
+  (* copied from [sim_refl] *)
+  revert m n.
+  cofix CH.
+  intros m n.
+  constructor. 
+  unfold simF. (* this was omitted in [sim_refl] *) 
+  intros m' a tr. 
+  exists m'. (* *)
+  split.
+  (* - exact tr. *)
+  (* - apply CH. Guarded. *)
+
+
+
+(* strong bisim, based upon [sim_refl] *)
+(* ! aborted since we are showing weak bisim for the existing example. *)
+Lemma bisim 
+  (* changed from [Set] to [Type] due to error. *) 
+  (* -- uncertain of impact, but recall D.CP. preferring [Set] *)
+  (M N A : Type) 
+  (LTS1 : M -> A -> M -> Prop)
+  (LTS2 : N -> A -> N -> Prop)
+  (m : M) (n : N) : sim lts bigstep g1 g1.
+Proof.
+  (* copied from [sim_refl] *)
+  revert m n.
+  cofix CH.
+  intros m n.
+  constructor. 
+  unfold simF. (* this was omitted in [sim_refl] *) 
+  intros m' a tr. 
+  exists m'. (* *)
+  split.
+  (* - exact tr. *)
+  (* - apply CH. Guarded. *)
+Abort.
+
+
